---
math: yes
title: "Quadratics & Completing the Square"
categories: ["MAT1340 - College Algebra", "Week 4"]
tags: [lecture]
description:
---

### Finding the Vertex of a Quadratic

For a quadratic function in standard form

$$f(x) = ax^2 + bx + c,$$

the vertex can be found in two steps:

1. Compute the axis of symmetry using
   $$
   x = -\frac{b}{2a}.
   $$

2. Plug this value into $f(x)$ to get the $y$-coordinate.

So the vertex is

$$
\left( -\tfrac{b}{2a}, \, f\!\left(-\tfrac{b}{2a}\right) \right).
$$

---

#### Example

Take $f(x)=3x^2+6x+9$. Here $a=3$, $b=6$, $c=9$.

The $x$-coordinate is:

$$
-\frac{6}{2 \cdot 3} = -1
$$

Now evaluate $f(-1)$:

$$
\begin{align*}
f(-1) &= 3(-1)^2 + 6(-1) + 9 \\
&= 3 - 6 + 9 \\
&= 6
\end{align*}
$$

So the vertex is at $\;(-1, 6)$.

---

### Completing the Square

Not all quadratics are easy to factor. For example:

$$
f(x) = -2x^2 - 12x - 24
$$

To rewrite such functions, we use **completing the square**.

---

#### General Idea

Start with a quadratic of the form

$$
x^2 + bx + c
$$

We add and subtract $\left(\tfrac{b}{2}\right)^2$:

$$
x^2 + bx + \colorbox{yellow}{$\left(\tfrac{b}{2}\right)^2$} - \colorbox{yellow}{$\left(\tfrac{b}{2}\right)^2$} + c
$$

The first three terms factor neatly:

$$
(x + \tfrac{b}{2})^2 - \left(\tfrac{b}{2}\right)^2 + c
$$

So weâ€™ve transformed

$$
x^2+bx+c \;\;\longrightarrow\;\; (x + \tfrac{b}{2})^2 - \left(\tfrac{b}{2}\right)^2 + c
$$

This is useful because it converts standard form into **vertex form**.

---

#### Example

Convert $f(x) = x^2 - 6x + 13$ into vertex form.

Here, $a=1$, $b=-6$, $c=13$.

Compute:

$$
\left(\tfrac{b}{2}\right)^2 = \left(\tfrac{-6}{2}\right)^2 = (-3)^2 = 9
$$

Add and subtract 9:

$$
f(x) = x^2 - 6x + \colorbox{yellow}{$9 - 9$} + 13
$$

Factor and simplify:

$$
\begin{align*}
f(x) &= (x - 3)^2 - 9 + 13 \\
&= (x - 3)^2 + 4
\end{align*}
$$

So the vertex form is:

$$
f(x) = (x-3)^2 + 4
$$

From this, we see the vertex is at $\,(3,4)$.
