---
math: yes
title: "Deriving the Quadratic Formula"
categories: ["MAT1340 - College Algebra", "Week 4"]
tags: [lecture]
description:
---

We start with a quadratic equation of the form

$$
y = ax^2+bx+c
$$

where we want $y$ to be zero (to find the $x$--intercepts):

$$
ax^2+bx+c = 0
$$

We can divide by $a$ to remove the coefficient from the $x^2$ term:

$$
x^2+\frac{b}{a}x+\frac{c}{a} = 0
$$

Then, let's move the constant $\frac{c}{a}$ to the other side so that we don't have to deal with it:

$$
x^2+\frac{b}{a}x=-\frac{c}{a}
$$

Now we can complete the square (remember: to complete the square, we take the coefficient attached to the $x$, divide by $2$, and square):

$$
x^2+\frac{b}{a}x + \left( \frac{b}{2a} \right)^2 - \left( \frac{b}{2a} \right)^2 = -\frac{c}{a}
$$

We can factor now:

$$
\left( x+\frac{b}{2a} \right)^2 - \left( \frac{b}{2a} \right)^2 = -\frac{c}{a}
$$

Now, we can rearrange to solve for $x$:

$$
\begin{align*}
\left( x+\frac{b}{2a} \right)^2 &= \left( \frac{b}{2a} \right)^2-\frac{c}{a} \\
\left( x+\frac{b}{2a} \right)^2 &= \frac{b^2}{4a^2} - \frac{c}{a} \\
\left( x+\frac{b}{2a} \right)^2 &= \frac{b^2}{4a^2} - \frac{4ac}{4a^2} \\
\left( x+\frac{b}{2a} \right)^2 &= \frac{b^2-4ac}{4a^2} \\
x+\frac{b}{2a} &= \pm\sqrt{\frac{b^2-4ac}{4a^2}} \\
x+\frac{b}{2a} &= \frac{\pm \sqrt{b^2-4ac}}{\pm \sqrt{4a^2}} \\
x + \frac{b}{2a} &= \frac{\pm \sqrt{b^2-4ac}}{2a} \\
x &= \frac{-b}{2a} + \frac{\pm\sqrt{b^2-4ac}}{2a} \\
x &= \frac{-b \pm \sqrt{b^2-4ac}}{2a}
\end{align*}
$$
