---
math: yes
title: 6.5 - Length of Curves
description: "Derivation and application of the arc length formulae"
categories: [MAT2420, Lecture Notes]
---

## Introduction

![](/assets/images/MAT2420/6.5/6-5-1-light.svg){: .light }
![](/assets/images/MAT2420/6.5/6-5-1-dark.svg){: .dark }

What is the length of $f\left(x\right)$ on $\left[ a, b \right]$?

---

## Strategy for Finding Length

1. We can partition the interval $\left[ a, b \right]$ into $n$ equal–length subintervals,

    ![](/assets/images/MAT2420/6.5/6-5-2-light.svg){: .light }
    ![](/assets/images/MAT2420/6.5/6-5-2-dark.svg){: .dark }

    where $\Delta x$ is given by $\frac{b-a}{n}$.

2. At each subinterval, we can approximate the length of $f\left(x\right)$ by using a straight line segment.

    ![](/assets/images/MAT2420/6.5/6-5-3-light.svg){: .light }
    ![](/assets/images/MAT2420/6.5/6-5-3-dark.svg){: .dark }

    The length of the straight line segment joining $\left( x_{k-1}, f \left( x_{k-1} \right) \right)$ and $\left( x_{k}, f \left( x_{k} \right) \right)$ is given by

    $$
    \begin{align*}
    L &= \sqrt{ \left( x_{k} - x_{k-1} \right) ^{2} + \left( f \left( x_{k} \right) - f \left( x_{k-1} \right) ^{2} \right)  } \\
    &= \sqrt{ \left( \Delta x \right) ^{2} + \left( \Delta y \right) ^{2} }
    .\end{align*}
    $$

3. Repeat the same procedure for all $n$ subintervals, and sum all $n$ "linear approximations" to get an approximation for the length of $f\left(x\right)$ on $\left[ a, b \right]$.

    $$
    \begin{gather*}
    \sum_{j=1}^{n} \sqrt{ \left( \Delta x \right) ^{2} + \left( \Delta y \right) ^{2} } \\
    \text{as}~ \Delta x \to 0, ~ \text{it becomes} ~ \,\mathrm{d}x, \\
    \text{as}~ \Delta y \to 0, ~ \text{it becomes} ~ \,\mathrm{d}y
    .\end{gather*}
    $$

4. Make the partition of $\left[ a, b \right]$ "finer;" that is, let $\Delta x \to 0$. Then, since $\Delta x \to 0$ is equivalent to $n \to \infty$,

    $$
    \lim_{ n \to \infty } \sum_{j=1}^{n} \sqrt{ \left( \Delta x \right) ^{2} + \left( \Delta y \right) ^{2} } \to \int_{a}^{b} \sqrt{ \left( \mathrm{d}x \right) ^{2} + \left( \mathrm{d}y \right) ^{2} }
    .
    $$

5. Now, we can manipulate $\int_{a}^{b} \sqrt{ \left( \left( \mathrm{d}x \right)^{2} + \left( \mathrm{d}y \right)^{2} \right) }$ so that it involves only $\mathrm{d}x$ or only $\mathrm{d}y$.

    $$
    \begin{align*}
    \int_{a}^{b} \sqrt{ \left( 1 + \frac{ \left( \mathrm{d}y \right) ^{2}}{ \left( \mathrm{d}x \right) ^{2}} \right) \left( \mathrm{d}x \right) ^{2} }
    &= \int_{a}^{b} \sqrt{ 1 + \left( \frac{\mathrm{d}y}{\mathrm{d}x} \right) ^{2} } \sqrt{ \left( \mathrm{d}x \right) ^{2} } \\
    &= \int_{a}^{b} \sqrt{ 1 + f'\left( x \right) ^{2} } \,\mathrm{d}x
    .\end{align*}
    $$

> Arc Length Formulae
>
> $$
> \begin{align*}
> L &= \int_{a}^{b} \sqrt{ 1 + f'\left( x \right) ^{2} } \,\mathrm{d}x \\
> L &= \int_{c}^{d} \sqrt{ 1 + f'\left(y\right)^{2} } \,\mathrm{d}y
> .\end{align*}
> $$
{: .prompt-info }

---

## Example Problem

> Problem 1
>
> Find the arc length of the curve
>
> $$
> y = \ln \left( x - \sqrt{ x^{2}-1 } \right)
> $$
>
> over $1 \leq x \leq \sqrt{ 122 }$.
{: .prompt-warning }

First we'll rewrite, solving for $x$.

$$
\begin{align*}
e^{y} &= x - \sqrt{ x^{2} - 1 } \\
-\left( e^{y} - x \right) &= \sqrt{ x^{2}-1 } \\
\left( -e^{y}+x \right) ^{2} &= x^{2} - 1 \\
e^{2y} - 2xe^{y} + x^{2} &= x^{2}-1 \\
e^{2y} - 2xe^{y} &= -1 \\
2xe^{y} &= 1+e^{2y} \\
x &= \frac{1+e^{2y}}{2e^{y}} \\
x &= \frac{1}{2} \left( \frac{1}{e^{y}} + \frac{e^{2y}}{e^{y}} \right)  \\
g\left(y\right) &= x = \frac{1}{2} \left( e^{y}+e^{-y} \right)
.\end{align*}
$$

Then, translate the integration interval to the $y$–axis.

$$
\begin{align*}
f\left(x\right) &= \ln \left( x-\sqrt{ x^{2}-1 } \right) \\
c &= f \left( 1 \right) = 0 \\
d &= f \left( \sqrt{ 122 } \right) = \ln \left( \sqrt{ 122 } - 11 \right)
.\end{align*}
$$

Now, we'll take the derivative of this function and square it, in preparation for substitution into the previously derived Arc Length Formulae.

$$
\begin{align*}
\frac{\mathrm{d}}{\mathrm{d}x} \,g\left(y\right) &= \frac{1}{2} \left( e^{y} - e^{-y} \right) \\
\left( g'\left(y\right) \right) ^{2} &= \frac{1}{4} \left( e^{2y} - 2 + e^{-2y} \right)
.\end{align*}
$$

Finally, perform the substitution and integrate.

$$
\begin{align*}
L &= \int_{0}^{\ln \left( \sqrt{ 122 } - 11 \right) } \sqrt{ 1 + \left( \frac{1}{4} \left( e^{2y} - 2 + e^{-2y} \right) \right)  } \,\mathrm{d}y \\
&= \int_{0}^{\ln \left( \sqrt{ 122 } - 11 \right) } \sqrt{ 1 + \left( \frac{1}{4} e^{2y} - \frac{1}{2} + \frac{1}{4}e^{-2y} \right)  } \,\mathrm{d}y \\
&= \int_{0}^{\ln \left( \sqrt{ 122 }-11 \right) } \sqrt{ \underbrace{\frac{1}{4}e^{2y}+\frac{1}{2}+\frac{1}{4}e^{-2y}}_{\text{Perfect Square}} } \,\mathrm{d}y \\
&= \int_{0}^{\ln \left( \sqrt{ 122 }-11 \right) } \sqrt{ \left( \frac{1}{2}e^{y}+\frac{1}{2}e^{-y} \right) ^{2} } \,\mathrm{d}y \\
&= \int_{0}^{\ln \left(  \sqrt{ 122 }-11 \right) } \left( \frac{1}{2} e^{y} + \frac{1}{2} e^{-y} \right)  \,\mathrm{d}y \\
&= \frac{1}{2} \int_{0}^{\ln \left( \sqrt{ 122 }-11 \right) } \left( e^{y} + e^{-y} \right)  \,\mathrm{d}y \\
&= \frac{1}{2} \left[ e^{y}-e^{-y} \right] _{0}^{\ln \left( \sqrt{ 122 }-11 \right) } \\
&= \frac{1}{2} \left[ \left( e^{\ln \left( \sqrt{ 122 }-11 \right) }-e^{-\ln \left( \sqrt{ 122 }-11 \right) } \right)^{2} -\left( e^{0}-e^{-0} \right)  \right]   \\
&= \frac{1}{2} \left[ \sqrt{ 122 }-11 - \frac{1}{\sqrt{ 122 }-11}  \right] \\
&= \frac{1}{2} \left[ \frac{\left( \sqrt{ 122 }-11 \right) ^{2}}{\sqrt{ 122 } - 11} - \frac{1}{\sqrt{ 122 }-11}\right]  \\
&= \frac{1}{2}\left[ \frac{\left( \sqrt{ 122 }-11 \right) ^{2}-1}{\sqrt{ 122 }-11} \right]  \\
&= \frac{1}{2} \left[ \frac{122-22\sqrt{ 122 }+121}{\sqrt{ 122 }-11} \right]  \\
&= \frac{1}{2} \left[ \frac{242-22\sqrt{ 122 }}{\sqrt{ 122 }-11} \right]  \\
&= \frac{1}{2} \left[ \frac{-22 \left( \sqrt{ 122 } - 11 \right) }{\sqrt{ 122 }-11} \right]  \\
&= \frac{1}{2} \cdot -22 \\
&= \boxed{-11}
.\end{align*}
$$
