---
math: yes
title: "9.4 - Linear ODE Integrating Factor"
description: "Master the method of integrating factors to solve first-order linear differential equations, and see it in action through worked examples—including Newton’s Law of Cooling and a classic initial value problem."
categories: [MAT2420, Lecture Notes]
---

## Method to solve 1<sup>st</sup> order linear ODEs: Integrating Factors

$$
y'(t) + P(t) y = f(t)
\tag{1}
.
$$

> Key Idea
>
> Recall the product rule. The left–hand side of $(1)$ kind of looks like the derivative of a product. In other words, is it possible to make the left–hand side the derivative of a product?
{: .prompt-info }

In order to do so, we can multiply both sides of $(1)$ by an unknown differentiable function $u(t)$.

$$
u(t)y'(t) + u(t)P(t)y = u(t)f(t)
\tag{2}
$$

Then, in order for$\frac{d}{\,\mathrm{d}t}(u(t)y(t))$ to equal the left–hand side of $(2)$, it must be the case that

$$
u' = u(t) P(t)
$$

$$
\begin{align*}
\frac{\mathrm{d}u}{\mathrm{d}t} = u(t) P(t) && \text{where} \, u(t) \, \text{is unknown}
.\end{align*}
$$

This is a separable $1^{\text{st}}$ order ODE.

$$
\begin{align*}
\frac{1}{u(t)} \,\mathrm{d}u &= P(t) \,\mathrm{d}t \\
\int \frac{1}{u(t)} \,\mathrm{d}u &= \int P(t) \,\mathrm{d}t \\
\ln |u(t)| &= \int P(t) \,\mathrm{d}t \\
\end{align*}
$$

Now we can solve for $u(t)$.

$$
\begin{align*}
u(t) = e^{\int P(t) \,\mathrm{d}t}
\tag{3}
.\end{align*}
$$

$(3)$ is called an "integrating factor." Now we need to solve $\frac{\mathrm{d}y}{\mathrm{d}t} + P(t)y = f(t)$ using this integrating factor.

1. Compute the integrating factor.

    $$
    u(t) = e^{\int P(t) \,\mathrm{d}t}
    .
    $$

2. Multiply both sides of standard form by the integrating factor $u(t)$.

    $$
    \begin{align*}
    u(t) \frac{\mathrm{d}y}{\mathrm{d}t} + u(t) P(t) y &= u(t) f(t) \\
    \frac{d}{\,\mathrm{d}t} (u(t) y(t)) &= u(t)f(t) \\
    e^{\int P(t) \,\mathrm{d}t} y(t) &= e^{\int P(t) \,\mathrm{d}t} y' + e^{\int P(t) \,\mathrm{d}t} P(t) y
    .\end{align*}
    $$

    Then, integrating with respect to $t$,

    $$
    \begin{align*}
    \int \frac{d}{\mathrm{d}t} \left( u(t) y(t) \right) \,\mathrm{d}t &= \int u(t) f(t) \,\mathrm{d}t \\
    u(t) y(t) &= \int u(t) f(t) \,\mathrm{d}t \\
    y(t) &= \frac{1}{u(t)} \int u(t) f(t) \,\mathrm{d}t + \frac{C}{u(t)}
    .\end{align*}
    $$

---

### Example—9.4 Question 3

Solve the following initial value problem.

$$
y'(t)-6y=12, \quad y(0) = 0
.
$$

1. Recall the standard form and integrating factor:

    $$
    \begin{align*}
    y' + P(t)y &= f(t) \\
    u(t) &= e^{\ln P(t) \,\mathrm{d}t}
    .\end{align*}
    $$

    So the integrating factor for the problem is

    $$
    u(t)=e^{\int -6 \,\mathrm{d}t} = e^{-6t}
    .
    $$

2. Multiply both sides of the ODE by $u(t)$:

    $$
    \begin{align*}
    e^{-6t} y' - 6e^{-6t} y &= 12e^{-6t}
    .\end{align*}
    $$

    This is easily recognizable as the derivative of a product, namely $e^{-6t} y(t)$. Therefore,

    $$
    \begin{align*}
    \int \frac{d}{\,\mathrm{d}t} \left( e^{-6t} y(t) \right)  \,\mathrm{d}t &= 12 \int e^{-6t} \,\mathrm{d}t \\
    e^{-6t} y(t) &= -2e^{-6t} + C
    .\end{align*}
    $$

    We can multiply both sides by $e^{-6t}$:

    $$
    \begin{align*}
    y(t) &= e^{6t} \left( -2e^{-6t} + C \right) \\
    &= -2 + Ce^{6t}
    .\end{align*}
    $$

    This is the general explicit family of solutions; we need to apply the given initial condition $y(0) = 0$.

    $$
    \begin{align*}
    0 &= -2 + Ce^{6(0)} \\
    2 &= C
    .\end{align*}
    $$

    Therefore, the solution is

    $$
    y(t)=-2+2e^{6t}
    .
    $$

> Note from Professor
>
> In the psets, the coefficients $P(t)$ and $f(t)$ in
>
> $$
> y' + P(t) y = f(t) \tag{4}, \quad \text{where}
> $$
>
> $$
> \begin{align*}
> P(t) &= -k \\
> f(t) &=  b
> \end{align*}
> $$
>
> are constants.
> In this situation, the solution to $(4)$ is
>
> $$
> y(t) = -\frac{b}{k} + Ce^{kt}
> .
> $$
{: .prompt-tip }

---

## Newton's Law of Cooling

The rate of heat loss (or gain) of a body is proportional to the difference between the body's temperature and the ambient temperature.

- Let $T(t)$ represent the temperature of the body at time $t$.
- Let $A$ represent the ambient temperature (assuming it is constant for the sake of simplicity).
- Let $k$ be a proportionality constant

Then, the "rate of heat loss or gain" or rate of change of heat for the body is given by

$$
\frac{\mathrm{d}T}{\mathrm{d}t} = k (T(t)-A).
$$

Of course, if the object is heating up $k > 0$, and if cooling down $k < 0$. For the demonstration, we will have $k < 0$.

$$
\frac{\,\mathrm{d}T}{\,\mathrm{d}t} = -k(T(t) - A)
.
$$

This is a separable $1^{\text{st}}$ order ODE.

$$
\begin{align*}
\frac{1}{T(t)-A} \,\mathrm{d}t &= -K \,\mathrm{d}t \\
\ln |T(t) - A| &= -kt + C
.\end{align*}
$$

Then we can solve for $T(t)$ by exponentiating both sides:

$$
\begin{align*}
T(t) - A &= e^{(-kt+C)} \\
T(t) - A &= e^{-kt}\underbrace{e^{C}}_{\text{constant}} \\
T(t) - A &= Ce^{-kt} \\
T(t) &= A + Ce^{-kt}
.\end{align*}
$$
